#Ãœbung #Mathe-Vorkurs 
## 22.
#### e)
$\huge{\frac{3-\frac{3a-b}{a+b}}{4\frac{a+b}{a-b}-\frac{16b^2}{a^2-b^2}-\frac{16b}{a+b}}}$
$\huge{=\frac{\frac{-3a+b}{a+b}+\frac{3a+3b}{a+b}}{\frac{4a^2+8ab+4b^2-16ab+16b^2-16b^2}{a^2-b^2}}}$
$\huge{=\frac{\frac{4b}{a+b}}{\frac{4a^2-8ab+4b^2}{a^2-b^2}}}$
$\huge{=\frac{4b*(a^2-b^2)}{(a+b)*(4a^2-8ab+4b^2)}}$
$\huge{=\frac{4a^2b-4b^3}{4a^3-8a^2b+4ab^2+4a^2b-8ab^2+4b^3}}$
$\huge{=\frac{4a^2b-4b^3}{4a^3-4a^2b-4ab^2+4b^3}}$
$\huge{=\frac{4*(a^2b-b^3)}{4*(a^3-a^2b-ab^2+b^3)}}$
$\huge{=\frac{a^2b-b^3}{a^3-a^2b-ab^2+b^3}}$
$\huge{=\frac{b*(a^2-b^2)}{a^2*(a-b)-b^2*(a-b)}}$
$\huge{=\frac{b*(a+b)*(a-b)}{(a^2-b^2)*(a-b)}}$
$\huge{=\frac{b*(a+b)*(a-b)}{(a+b)*(a-b)*(a-b)}}$
$\huge{=\frac{b}{a-b}}$